coq/proof/SoundPostcond.v
@@ -33,11 +33,15 @@ Lemma has_false_False
 Proof.
 Admitted.
 
+(* TODO: we can assume source's progress *)
+(* TODO: we need to split the cases: call and non-call. *)
 Lemma postcond_cmd_sound
       conf_src st0_src cmd_src cmds_src
       conf_tgt st0_tgt cmd_tgt cmds_tgt
       invst0 invmem0 inv0
       st1_tgt evt inv1
+      (NONCALL_SRC: ~ Instruction.isCallInst cmd_src)
+      (NONCALL_TGT: ~ Instruction.isCallInst cmd_tgt)
       (CMDS_SRC: st0_src.(EC).(CurCmds) = cmd_src :: cmds_src)
       (CMDS_TGT: st0_tgt.(EC).(CurCmds) = cmd_tgt :: cmds_tgt)
       (POSTCOND: Postcond.postcond_cmd cmd_src cmd_tgt inv0 = Some inv1)
@@ -46,7 +50,7 @@ Lemma postcond_cmd_sound
       (STEP_TGT: sInsn conf_tgt st0_tgt st1_tgt evt):
   exists st1_src invst1 invmem1,
     <<STEP_SRC: sInsn conf_src st0_src st1_src evt>> /\
-    <<STATE: InvState.Rel.sem conf_src conf_tgt st1_src st1_tgt invst1 invmem1 inv1>>/\
+    <<STATE: InvState.Rel.sem conf_src conf_tgt st1_src st1_tgt invst1 invmem1 inv1>> /\
     <<MEM: InvMem.Rel.sem conf_src conf_tgt st1_src.(Mem) st1_tgt.(Mem) invmem1>> /\
     <<MEMLE: InvMem.Rel.le invmem0 invmem1>>.
 Proof.
